Fix one proof

src/ExampleParser.v
@@ -509,7 +509,28 @@ Proof.
   reflexivity.
 Qed.
 
-Lemma replicate_length {P} `{Biparser P} {PL : PromonadLaws P} (n : nat)
+Lemma comap_bind_morph' {U U' A B} (f : U -> option U') (u : Product parser2 printer2 U' A) (k : A -> B)
+  : comap f (bind u (fun x => ret (k x))) = bind (comap f u) (fun x => ret (k x)).
+Proof.
+  cbn. unfold Profunctor_Product; cbn.
+  f_equal.
+  - apply functional_extensionality; intros s.
+    destruct (fst u s) as [ [] | ]; cbn; auto.
+  - apply functional_extensionality; intros s; cbn.
+    destruct (f s) as [ | ]; cbn; auto.
+    destruct (snd u u0) as [ [] | ]; cbn; auto.
+Qed.
+
+Class PLaw' P `{Biparser P} : Prop :=
+  plaw' : forall U U' A B (f : U -> option U') (u : P U' A) (k : A -> B),
+    comap f (bind u (fun x => ret (k x))) = bind (comap f u) (fun x => ret (k x)).
+
+Instance PLaw'_biparser : PLaw' (Product parser2 printer2).
+Proof.
+  exact @comap_bind_morph'.
+Qed.
+
+Lemma replicate_length {P} `{Biparser P} `{PLaw' P} {PL : PromonadLaws P} (n : nat)
   : replicate (P := P) n biparse_token >>= (fun x : list t => ret (List.length x))
   = replicate n biparse_token >>= (fun _ : list t => ret n).
 Proof.
@@ -518,11 +539,13 @@ Proof.
   - rewrite !bind_bind. f_equal. apply functional_extensionality. intros x.
     rewrite !bind_bind.
     transitivity (comap (P := P) tail (replicate n biparse_token >>= fun x => ret (length x)) >>= fun n => ret (S n)).
-    + admit.
-    + admit.
-Admitted.
+    + rewrite plaw'. rewrite !bind_bind. f_equal; apply functional_extensionality; intros xs.
+      rewrite 2 ret_bind. reflexivity.
+    + rewrite IHn. rewrite plaw', !bind_bind. f_equal; apply functional_extensionality; intros xs.
+      rewrite 2 ret_bind. reflexivity.
+Qed.
 
-Lemma replicate_length_ {P} `{Biparser P} {PL : PromonadLaws P} (n : nat)
+Lemma replicate_length_ {P} `{Biparser P} {PL : PromonadLaws P} `{!PLaw' P} (n : nat)
   : replicate (P := P) n biparse_token >>= (fun x : list t => ret (Some (List.length x)))
   = replicate n biparse_token >>= (fun _ : list t => ret (Some n)).
 Proof.
